Basicly valid
Working on timeouts

src/SDK/MessageBody.dfy
@@ -17,7 +17,6 @@ include "Serialize/HeaderAuth.dfy"
 include "Serialize/SerializeFunctions.dfy"
 include "../../libraries/src/Collections/Sequences/Seq.dfy"
 
-
 module MessageBody {
   // export
   //   provides EncryptMessageBody, DecryptFramedMessageBody, DecryptNonFramedMessageBody,
@@ -50,9 +49,9 @@ module MessageBody {
     case AADSingleBlock => BODY_AAD_CONTENT_SINGLE_BLOCK
   }
 
-  const START_SEQUENCE_NUMBER: uint32 := 1
-  const ENDFRAME_SEQUENCE_NUMBER: uint32 := 0xFFFF_FFFF
-  const NONFRAMED_SEQUENCE_NUMBER: uint32 := 1
+  const START_SEQUENCE_NUMBER: uint32 := Frames.START_SEQUENCE_NUMBER
+  const ENDFRAME_SEQUENCE_NUMBER: uint32 := Frames.ENDFRAME_SEQUENCE_NUMBER
+  const NONFRAMED_SEQUENCE_NUMBER: uint32 := Frames.NONFRAMED_SEQUENCE_NUMBER
 
   function method IVSeq(suite: Client.AlgorithmSuites.AlgorithmSuite, sequenceNumber: uint32)
     :(ret: seq<uint8>)
@@ -91,7 +90,7 @@ module MessageBody {
     && SumPlaintextSegments(plaintextSeg) == plaintext
   }
 
-  predicate FramesEncryptPlaintextSegments(frames: seq<MessageFrame>, plaintextSeg: seq<seq<uint8>>)
+  predicate FramesEncryptPlaintextSegments(frames: seq<Frame>, plaintextSeg: seq<seq<uint8>>)
   {
     // The total number of frames MUST equal the total number of plaintext segments.
     if |frames| != |plaintextSeg| then
@@ -102,9 +101,8 @@ module MessageBody {
         true
       else
         // Drop the segments
-        && FramesEncryptPlaintextSegments(frames[..|frames| - 1], plaintextSeg[..|frames| - 1])
-        && AESEncryption.CiphertextGeneratedWithPlaintext(frames[|frames| - 1].encContent, plaintextSeg[|frames| - 1])
-
+        && FramesEncryptPlaintextSegments(Seq.DropLast(frames), Seq.DropLast(plaintextSeg))
+        && AESEncryption.CiphertextGeneratedWithPlaintext(Seq.Last(frames).encContent, Seq.Last(plaintextSeg))
   }
 
   // // Steps for inductive proofs EncryptMessageBody
@@ -178,6 +176,13 @@ module MessageBody {
   || Frames.IsRegularFrame(frame)
   witness *
 
+  type Frame = frame: Frames.Frame
+  |
+  || Frames.IsFinalFrame(frame)
+  || Frames.IsRegularFrame(frame)
+  || Frames.IsFinalFrame(frame)
+  witness *
+
   lemma LemmaAddingNextRegularFrame(
     regularFrames: MessageRegularFrames,
     nextRegularFrame: Frames.RegularFrame
@@ -206,7 +211,7 @@ module MessageBody {
         // && (forall frame: Frame | frame in frames :: |frame.iv| == suite.encrypt.ivLength as int)
         // && FramesToSequence(frames) == seqWithGhostFrames.sequence
         // && FramesEncryptPlaintext(body, plaintext)
-        && (forall frame 
+        && (forall frame: Frames.RegularFrame
           | frame in body.regularFrames
           :: AESEncryption.EncryptedWithKey(frame.encContent, key))
         && AESEncryption.EncryptedWithKey(body.finalFrame.encContent, key)
@@ -234,7 +239,7 @@ module MessageBody {
       // invariant FramesToSequence(regularFrames) == body
       // invariant FramesEncryptPlaintextSegments(regularFrames, plaintextSeg) // Frames decrypt to chunks of plaintext
       // invariant SumPlaintextSegments(plaintextSeg) == plaintext[..n] // Chunks of plaintext sum up to plaintexts
-      invariant forall frame
+      invariant forall frame: Frames.RegularFrame
       | frame in regularFrames
       ::
         && AESEncryption.EncryptedWithKey(frame.encContent, key)
@@ -447,186 +452,234 @@ module MessageBody {
     return Success(finalFrame);
   }
 
-  // method DecryptFramedMessageBody(
-  //   rd: Streams.ByteReader,
-  //   suite: Client.AlgorithmSuites.AlgorithmSuite,
-  //   key: seq<uint8>,
-  //   frameLength: int,
-  //   messageID: Msg.MessageID
-  // )
-  //   returns (res: Result<seq<uint8>, string>)
-  //   requires rd.Valid()
-  //   requires |key| == suite.encrypt.keyLength as int
-  //   requires 0 < frameLength < UINT32_LIMIT
-  //   modifies rd.reader`pos
-  //   ensures rd.Valid()
-  //   ensures res.Success? ==> DecryptedWithKey(key, res.value)
-  //   ensures match res
-  //     case Failure(_) => true
-  //     case Success(plaintext) => //Exists a sequence of frames which encrypts the plaintext and is serialized in the read section of the stream
-  //       old(rd.reader.pos) <= rd.reader.pos <= |rd.reader.data|
-  //       && exists frames: seq<Frame> | |frames| < UINT32_LIMIT && (forall frame | frame in frames :: frame.Valid())
-  //           && FramesToSequence(frames) == rd.reader.data[old(rd.reader.pos)..rd.reader.pos] ::
-  //             && FramesEncryptPlaintext(frames, plaintext)
-  // {
-  //   var plaintext := [];
-  //   var n: uint32 := 1;
-  //   ghost var frames: seq<Frame> := [];
-  //   ghost var plaintextSeg: seq<seq<uint8>> := []; // Chuncks of plaintext which are decrypted from the frame
+  method DecryptFramedMessageBody(
+    body: FramedMessage,
+    key: seq<uint8>
+  )
+    returns (res: Result<seq<uint8>, string>)
+    // requires rd.Valid()
+    requires |key| == body.finalFrame.header.suite.encrypt.keyLength as int
+    // requires 0 < frameLength < UINT32_LIMIT
+    // modifies rd.reader`pos
+    // ensures rd.Valid()
+    // ensures res.Success? ==> DecryptedWithKey(key, res.value)
+    ensures match res
+      case Failure(_) => true
+      case Success(plaintext) => //Exists a sequence of frames which encrypts the plaintext and is serialized in the read section of the stream
+        // old(rd.reader.pos) <= rd.reader.pos <= |rd.reader.data|
+        // && exists frames: seq<Frame> | |frames| < UINT32_LIMIT && (forall frame | frame in frames :: frame.Valid())
+        //     && FramesToSequence(frames) == rd.reader.data[old(rd.reader.pos)..rd.reader.pos] ::
+        //       && FramesEncryptPlaintext(frames, plaintext)
+        && FramesEncryptPlaintext(body, plaintext)
+        && DecryptedWithKey(key, plaintext)
+  {
+    var plaintext := [];
+    // var n: uint32 := 1;
+    // // ghost var frames: seq<Frame> := [];
+    ghost var plaintextSeg: seq<seq<uint8>> := []; // Chuncks of plaintext which are decrypted from the frame
 
-  //   while true
-  //     decreases ENDFRAME_SEQUENCE_NUMBER - n
-  //     invariant rd.Valid()
-  //     invariant n as int - 1 == |frames|
-  //     invariant n <= ENDFRAME_SEQUENCE_NUMBER
-  //     invariant forall frame | frame in frames :: frame.Valid()
-  //     invariant old(rd.reader.pos) <= rd.reader.pos <= |rd.reader.data|
-  //     invariant FramesToSequence(frames) == rd.reader.data[old(rd.reader.pos)..rd.reader.pos]
-  //     invariant rd.Valid()
-  //     invariant FramesEncryptPlaintextSegments(frames, plaintextSeg) // All decrypted frames decrypt to the list of plaintext chuncks
-  //     invariant SumPlaintextSegments(plaintextSeg) == plaintext // The current decrypted frame is the sum of all decrypted chuncks
-  //     invariant DecryptedSegmentsWithKey(key, plaintextSeg)
-  //     invariant plaintext == SumPlaintextSegments(plaintextSeg)
-  //   {
-  //     assert {:split_here} true;
-  //     var frameWithGhostSeq :- DecryptFrame(rd, suite, key, frameLength, messageID, n);
-  //     assert |frameWithGhostSeq.sequence| < UINT32_LIMIT;
-  //     var decryptedFrame := frameWithGhostSeq.frame;
-  //     ghost var ciphertext := frameWithGhostSeq.sequence;
-  //     assert |ciphertext| < UINT32_LIMIT;
-  //     ghost var encryptedFrame := if decryptedFrame.FinalFrame? then
-  //       FinalFrame(decryptedFrame.seqNum, decryptedFrame.iv, ciphertext, decryptedFrame.authTag)
-  //     else
-  //       RegularFrame(decryptedFrame.seqNum, decryptedFrame.iv, ciphertext, decryptedFrame.authTag);
-  //     assert encryptedFrame.Valid();
-  //     frames := frames + [encryptedFrame];
+    // while true
+    //   decreases ENDFRAME_SEQUENCE_NUMBER - n
+    //   invariant rd.Valid()
+    //   invariant n as int - 1 == |frames|
+    //   invariant n <= ENDFRAME_SEQUENCE_NUMBER
+    //   invariant forall frame | frame in frames :: frame.Valid()
+    //   invariant old(rd.reader.pos) <= rd.reader.pos <= |rd.reader.data|
+    //   invariant FramesToSequence(frames) == rd.reader.data[old(rd.reader.pos)..rd.reader.pos]
+    //   invariant rd.Valid()
+    //   invariant FramesEncryptPlaintextSegments(frames, plaintextSeg) // All decrypted frames decrypt to the list of plaintext chuncks
+    //   invariant SumPlaintextSegments(plaintextSeg) == plaintext // The current decrypted frame is the sum of all decrypted chuncks
+    //   invariant DecryptedSegmentsWithKey(key, plaintextSeg)
+    //   invariant plaintext == SumPlaintextSegments(plaintextSeg)
+    // {
+    //   // assert {:split_here} true;
+    //   var frameWithGhostSeq :- DecryptFrame(rd, suite, key, frameLength, messageID, n);
+    //   assert |frameWithGhostSeq.sequence| < UINT32_LIMIT;
+    //   var decryptedFrame := frameWithGhostSeq.frame;
+    //   ghost var ciphertext := frameWithGhostSeq.sequence;
+    //   assert |ciphertext| < UINT32_LIMIT;
+    //   ghost var encryptedFrame := if decryptedFrame.FinalFrame? then
+    //     FinalFrame(decryptedFrame.seqNum, decryptedFrame.iv, ciphertext, decryptedFrame.authTag)
+    //   else
+    //     RegularFrame(decryptedFrame.seqNum, decryptedFrame.iv, ciphertext, decryptedFrame.authTag);
+    //   assert encryptedFrame.Valid();
+    //   frames := frames + [encryptedFrame];
 
-  //     var (decryptedFramePlaintext, final) := (decryptedFrame.encContent, decryptedFrame.FinalFrame?);
-  //     plaintext := plaintext + decryptedFramePlaintext;
-  //     plaintextSeg := plaintextSeg + [decryptedFramePlaintext];
-  //     if final {
-  //       assert FramesEncryptPlaintextSegments(frames, plaintextSeg);
-  //       assert SumPlaintextSegments(plaintextSeg) == plaintext;
-  //       break;
-  //     }
+    //   var (decryptedFramePlaintext, final) := (decryptedFrame.encContent, decryptedFrame.FinalFrame?);
+    //   plaintext := plaintext + decryptedFramePlaintext;
+    //   plaintextSeg := plaintextSeg + [decryptedFramePlaintext];
+    //   if final {
+    //     assert FramesEncryptPlaintextSegments(frames, plaintextSeg);
+    //     assert SumPlaintextSegments(plaintextSeg) == plaintext;
+    //     break;
+    //   }
 
-  //     n := n + 1;
-  //   }
-  //   assert |frames| < UINT32_LIMIT ;
-  //   assert (forall frame | frame in frames :: frame.Valid()) ;
-  //   assert FramesToSequence(frames) == rd.reader.data[old(rd.reader.pos)..rd.reader.pos];
-  //   return Success(plaintext);
-  // }
+    //   n := n + 1;
+    // }
 
-  // method DecryptFrame(
-  //   rd: Streams.ByteReader,
-  //   suite: Client.AlgorithmSuites.AlgorithmSuite,
-  //   key: seq<uint8>,
-  //   frameLength: int,
-  //   messageID: Msg.MessageID,
-  //   expectedSequenceNumber: uint32
-  // )
-  //   returns (res: Result<FrameWithGhostSeq, string>)
-  //   requires rd.Valid()
-  //   requires |key| == suite.encrypt.keyLength as int
-  //   requires 0 < frameLength < UINT32_LIMIT
-  //   modifies rd.reader`pos
-  //   ensures rd.Valid()
-  //   ensures match res // If the expected sequence number is the end frame sequence number then the frame is the final frame. However, the final frame can arrive earlier
-  //     case Success(frameWithGhostSeq) =>
-  //       expectedSequenceNumber == ENDFRAME_SEQUENCE_NUMBER ==> frameWithGhostSeq.frame.FinalFrame?
-  //     case Failure(_) => true
-  //   ensures res.Success? ==> |res.value.sequence| < UINT32_LIMIT
-  //   ensures match res
-  //     case Success(frameWithGhostSeq) => ( // Decrypting the frame encoded in the stream is the returned ghost frame
-  //       && var decryptedFrame := frameWithGhostSeq.frame;
-  //          var ciphertext := frameWithGhostSeq.sequence;
-  //          var final := decryptedFrame.FinalFrame?;
-  //          decryptedFrame.Valid()
-  //       && old(rd.reader.pos) < rd.reader.pos <= |rd.reader.data|
-  //       && AESEncryption.CiphertextGeneratedWithPlaintext(ciphertext, decryptedFrame.encContent)
-  //       && AESEncryption.DecryptedWithKey(key, decryptedFrame.encContent)
-  //       && var encryptedFrame := (if decryptedFrame.FinalFrame? then
-  //            FinalFrame(decryptedFrame.seqNum, decryptedFrame.iv, ciphertext, decryptedFrame.authTag)
-  //          else
-  //            RegularFrame(decryptedFrame.seqNum, decryptedFrame.iv, ciphertext, decryptedFrame.authTag));
-  //          rd.reader.data[old(rd.reader.pos)..rd.reader.pos] == FrameToSequence(encryptedFrame)
-  //       && AESEncryption.CiphertextGeneratedWithPlaintext(encryptedFrame.encContent, decryptedFrame.encContent))
-  //     case Failure(_) => true
-  // {
-  //   var final := false;
-  //   var sequenceNumber :- rd.ReadUInt32();
-  //   ghost var frameSerialization := UInt32ToSeq(sequenceNumber);
-  //   assert rd.reader.data[old(rd.reader.pos)..rd.reader.pos] == frameSerialization;
+    for i := 0 to |body.regularFrames|
+      // The goal is to assert FramesEncryptPlaintext.
+      // But this requires the final frame e.g. a FramedMessage.
+      // So I decompose this predicate into its parts
+      invariant |body.regularFrames[..i]| == |plaintextSeg|
+      invariant forall j
+      | 0 < j < i
+      :: AESEncryption.CiphertextGeneratedWithPlaintext(body.regularFrames[j].encContent, plaintextSeg[j]);
+      invariant FramesEncryptPlaintextSegments(body.regularFrames[..i], plaintextSeg) // So far: All decrypted frames decrypt to the list of plaintext chunks
+      invariant SumPlaintextSegments(plaintextSeg) == plaintext // So far: The current plaintext is the sum of all decrypted chunks
+      invariant DecryptedSegmentsWithKey(key, plaintextSeg)
+    {
+      var plaintextSegment :- DecryptFrame(body.regularFrames[i], key);
 
-  //   if sequenceNumber == ENDFRAME_SEQUENCE_NUMBER {
-  //     final := true;
-  //     sequenceNumber :- rd.ReadUInt32();
-  //     frameSerialization := frameSerialization + UInt32ToSeq(sequenceNumber);
-  //     assert rd.reader.data[old(rd.reader.pos)..rd.reader.pos] == frameSerialization;
-  //   }
+      assert FramesEncryptPlaintextSegments(body.regularFrames[..i], plaintextSeg);
+      assert AESEncryption.CiphertextGeneratedWithPlaintext(body.regularFrames[i].encContent, plaintextSegment);
+      assert FramesEncryptPlaintextSegments(body.regularFrames[..i] + [body.regularFrames[i]], plaintextSeg + [plaintextSegment]);
 
-  //   if sequenceNumber != expectedSequenceNumber {
-  //     return Failure("unexpected frame sequence number");
-  //   }
+      plaintext := plaintext + plaintextSegment;
+      plaintextSeg := plaintextSeg + [plaintextSegment];
 
-  //   assert {:focus} true;
-  //   var iv :- rd.ReadBytes(suite.encrypt.ivLength as int);
-  //   frameSerialization := frameSerialization + iv;
-  //   assert rd.reader.data[old(rd.reader.pos)..rd.reader.pos] == frameSerialization;
+      assert body.regularFrames[..i] + [body.regularFrames[i]] == body.regularFrames[..i + 1];
+      assert FramesEncryptPlaintextSegments(body.regularFrames[..i + 1], plaintextSeg);
+    }
 
-  //   var len := frameLength as uint32;
-  //   if final {
-  //     len :- rd.ReadUInt32();
-  //     if len > frameLength as uint32 {
-  //       return Failure("Final frame too long");
-  //     }
-  //     frameSerialization := frameSerialization + UInt32ToSeq(len);
-  //   }
+    var finalPlaintextSegment :- DecryptFrame(body.finalFrame, key);
+    plaintext := plaintext + finalPlaintextSegment;
 
-  //   var aad := BodyAAD(messageID, if final then AADFinalFrame else AADRegularFrame, sequenceNumber, len as uint64);
+    // assert |frames| < UINT32_LIMIT ;
+    // assert (forall frame | frame in frames :: frame.Valid()) ;
+    // assert FramesToSequence(frames) == rd.reader.data[old(rd.reader.pos)..rd.reader.pos];
+    return Success(plaintext);
+  }
 
-  //   assert {:focus} true;
-  //   var ciphertext :- rd.ReadBytes(len as nat);
-  //   frameSerialization := frameSerialization + ciphertext;
-  //   assert rd.reader.data[old(rd.reader.pos)..rd.reader.pos] == frameSerialization;
+  method DecryptFrame(
+    frame: Frame,
+    key: seq<uint8>
+    // ,expectedSequenceNumber: uint32
+  )
+    returns (res: Result<Uint8Seq32, string>)
+    // requires rd.Valid()
+    requires |key| == frame.header.suite.encrypt.keyLength as int
+    // requires 0 < frameLength < UINT32_LIMIT
+    // modifies rd.reader`pos
+    // ensures rd.Valid()
+    // ensures match res // If the expected sequence number is the end frame sequence number then the frame is the final frame. However, the final frame can arrive earlier
+    //   case Success(frameWithGhostSeq) =>
+    //     expectedSequenceNumber == ENDFRAME_SEQUENCE_NUMBER ==> frameWithGhostSeq.frame.FinalFrame?
+    //   case Failure(_) => true
+    // ensures res.Success? ==> |res.value| < UINT32_LIMIT
+    ensures match res
+      case Success(plaintextSegment) => ( // Decrypting the frame encoded in the stream is the returned ghost frame
+        // && var decryptedFrame := frameWithGhostSeq.frame;
+        //    var ciphertext := frameWithGhostSeq.sequence;
+        //    var final := decryptedFrame.FinalFrame?;
+        //    decryptedFrame.Valid()
+        // && old(rd.reader.pos) < rd.reader.pos <= |rd.reader.data|
+        && AESEncryption.CiphertextGeneratedWithPlaintext(frame.encContent, plaintextSegment)
+        && AESEncryption.DecryptedWithKey(key, plaintextSegment)
+      //   && var encryptedFrame := (if decryptedFrame.FinalFrame? then
+      //        FinalFrame(decryptedFrame.seqNum, decryptedFrame.iv, ciphertext, decryptedFrame.authTag)
+      //      else
+      //        RegularFrame(decryptedFrame.seqNum, decryptedFrame.iv, ciphertext, decryptedFrame.authTag));
+      //      rd.reader.data[old(rd.reader.pos)..rd.reader.pos] == FrameToSequence(encryptedFrame)
+      //   && AESEncryption.CiphertextGeneratedWithPlaintext(encryptedFrame.encContent, decryptedFrame.encContent)
+      )
+      case Failure(_) => true
+  {
+    // var final := false;
+    // var sequenceNumber :- rd.ReadUInt32();
+    // ghost var frameSerialization := UInt32ToSeq(sequenceNumber);
+    // assert rd.reader.data[old(rd.reader.pos)..rd.reader.pos] == frameSerialization;
 
-  //   var authTag :- rd.ReadBytes(suite.encrypt.tagLength as int);
-  //   frameSerialization := frameSerialization + authTag;
-  //   assert rd.reader.data[old(rd.reader.pos)..rd.reader.pos] == frameSerialization;
+    // if sequenceNumber == ENDFRAME_SEQUENCE_NUMBER {
+    //   final := true;
+    //   sequenceNumber :- rd.ReadUInt32();
+    //   frameSerialization := frameSerialization + UInt32ToSeq(sequenceNumber);
+    //   assert rd.reader.data[old(rd.reader.pos)..rd.reader.pos] == frameSerialization;
+    // }
 
-  //   var plaintext :- Decrypt(ciphertext, authTag, suite, iv, key, aad);
-  //   assert AESEncryption.CiphertextGeneratedWithPlaintext(ciphertext, plaintext);
-  //   assert rd.reader.data[old(rd.reader.pos)..rd.reader.pos] == frameSerialization;
+    // if sequenceNumber != expectedSequenceNumber {
+    //   return Failure("unexpected frame sequence number");
+    // }
 
-  //   var frame := if final then
-  //       FinalFrame(sequenceNumber, iv, plaintext, authTag)
-  //     else
-  //       RegularFrame(sequenceNumber, iv, plaintext, authTag);
+    // assert {:focus} true;
+    // var iv :- rd.ReadBytes(suite.encrypt.ivLength as int);
+    // frameSerialization := frameSerialization + iv;
+    // assert rd.reader.data[old(rd.reader.pos)..rd.reader.pos] == frameSerialization;
 
-  //   ghost var encryptedFrame := if final then
-  //       FinalFrame(sequenceNumber, iv, ciphertext, authTag)
-  //     else
-  //       RegularFrame(sequenceNumber, iv, ciphertext, authTag);
+    // var len := frameLength as uint32;
+    // if final {
+    //   len :- rd.ReadUInt32();
+    //   if len > frameLength as uint32 {
+    //     return Failure("Final frame too long");
+    //   }
+    //   frameSerialization := frameSerialization + UInt32ToSeq(len);
+    // }
 
-  //   // Feed dafny facts about the content of the stream
-  //   // Show dafny that the serialized frame is frameSerialization
-  //   assert frameSerialization == FrameToSequence(encryptedFrame);
+    var aad := BodyAADForFrame(frame);
 
-  //   // Prove read content of stream is frameSerialization
-  //   assert {:focus} true;
-  //   assert !final ==> frameSerialization[..4] == rd.reader.data[old(rd.reader.pos)..][..4];
-  //   assert !final ==> frameSerialization[4..][..suite.encrypt.ivLength as int] == rd.reader.data[old(rd.reader.pos)..][4..][..suite.encrypt.ivLength as int];
-  //   assert !final ==> frameSerialization[4 + suite.encrypt.ivLength as int..][..frameLength] == rd.reader.data[old(rd.reader.pos)..][4 + suite.encrypt.ivLength as int..][..frameLength];
-  //   assert !final ==> frameSerialization[4 + frameLength + suite.encrypt.ivLength as int..] == rd.reader.data[old(rd.reader.pos)..][4 + frameLength + suite.encrypt.ivLength as int..][..suite.encrypt.tagLength as int];
+    // assert {:focus} true;
+    // var ciphertext :- rd.ReadBytes(len as nat);
+    // frameSerialization := frameSerialization + ciphertext;
+    // assert rd.reader.data[old(rd.reader.pos)..rd.reader.pos] == frameSerialization;
 
-  //   // Prove equivalence frameSerialization and content read on the stream
-  //   assert rd.reader.data[old(rd.reader.pos)..rd.reader.pos] == frameSerialization;
+    // var authTag :- rd.ReadBytes(suite.encrypt.tagLength as int);
+    // frameSerialization := frameSerialization + authTag;
+    // assert rd.reader.data[old(rd.reader.pos)..rd.reader.pos] == frameSerialization;
 
-  //   assert old(rd.reader.pos) < rd.reader.pos <= |rd.reader.data|;
+    var plaintextSegment :- AESEncryption.AESDecrypt(
+      frame.header.suite.encrypt,
+      key,
+      frame.encContent,
+      frame.authTag,
+      frame.iv,
+      aad
+    );
 
-  //   return Success(FrameWithGhostSeq(frame,ciphertext));
-  // }
+    // assert AESEncryption.CiphertextGeneratedWithPlaintext(ciphertext, plaintext);
+    // assert rd.reader.data[old(rd.reader.pos)..rd.reader.pos] == frameSerialization;
+
+    // var frame := if final then
+    //     FinalFrame(sequenceNumber, iv, plaintext, authTag)
+    //   else
+    //     RegularFrame(sequenceNumber, iv, plaintext, authTag);
+
+    // ghost var encryptedFrame := if final then
+    //     FinalFrame(sequenceNumber, iv, ciphertext, authTag)
+    //   else
+    //     RegularFrame(sequenceNumber, iv, ciphertext, authTag);
+
+    // // Feed dafny facts about the content of the stream
+    // // Show dafny that the serialized frame is frameSerialization
+    // assert frameSerialization == FrameToSequence(encryptedFrame);
+
+    // // Prove read content of stream is frameSerialization
+    // assert {:focus} true;
+    // assert !final ==> frameSerialization[..4] == rd.reader.data[old(rd.reader.pos)..][..4];
+    // assert !final ==> frameSerialization[4..][..suite.encrypt.ivLength as int] == rd.reader.data[old(rd.reader.pos)..][4..][..suite.encrypt.ivLength as int];
+    // assert !final ==> frameSerialization[4 + suite.encrypt.ivLength as int..][..frameLength] == rd.reader.data[old(rd.reader.pos)..][4 + suite.encrypt.ivLength as int..][..frameLength];
+    // assert !final ==> frameSerialization[4 + frameLength + suite.encrypt.ivLength as int..] == rd.reader.data[old(rd.reader.pos)..][4 + frameLength + suite.encrypt.ivLength as int..][..suite.encrypt.tagLength as int];
+
+    // // Prove equivalence frameSerialization and content read on the stream
+    // assert rd.reader.data[old(rd.reader.pos)..rd.reader.pos] == frameSerialization;
+
+    // assert old(rd.reader.pos) < rd.reader.pos <= |rd.reader.data|;
+
+    // return Success(FrameWithGhostSeq(frame,ciphertext));
+    return Success(plaintextSegment);
+  }
+
+  method BodyAADForFrame(
+    frame: Frame
+  )
+    returns (aad: seq<uint8>)
+  {
+    var (sequenceNumber, bc, length) := match frame
+      case RegularFrame(header,seqNum,_,_,_) => (seqNum, AADRegularFrame, header.body.frameLength as uint64)
+      case FinalFrame(_,seqNum,_, encContent,_) => (seqNum, AADFinalFrame, |encContent| as uint64)
+      case NonFramed(_,_,encContent,_) => (NONFRAMED_SEQUENCE_NUMBER, AADSingleBlock, |encContent| as uint64);
+
+    aad := BodyAAD(frame.header.body.messageId, bc, sequenceNumber, length);
+  }
 
   method BodyAAD(messageID: seq<uint8>, bc: BodyAADContent, sequenceNumber: uint32, length: uint64) returns (aad: seq<uint8>) {
     var contentAAD := UTF8.Encode(BodyAADContentTypeString(bc));
@@ -655,19 +708,19 @@ module MessageBody {
   //   assert res.Success? ==> AESEncryption.DecryptedWithKey(key, res.value);
   // }
 
-  // predicate DecryptedWithKey(key: seq<uint8>, plaintext: seq<uint8>)
-  // {
-  //   if AESEncryption.DecryptedWithKey(key, plaintext) then true else
-  //     exists plaintextSeg | SumPlaintextSegments(plaintextSeg) == plaintext ::
-  //       DecryptedSegmentsWithKey(key, plaintextSeg)
-  // }
+  predicate DecryptedWithKey(key: seq<uint8>, plaintext: seq<uint8>)
+  {
+    if AESEncryption.DecryptedWithKey(key, plaintext) then true else
+      exists plaintextSeg | SumPlaintextSegments(plaintextSeg) == plaintext ::
+        DecryptedSegmentsWithKey(key, plaintextSeg)
+  }
 
-  // predicate DecryptedSegmentsWithKey(key: seq<uint8>, plaintextSeg: seq<seq<uint8>>)
-  // {
-  //   if plaintextSeg == [] then true else
-  //     && DecryptedSegmentsWithKey(key, plaintextSeg[..|plaintextSeg| - 1])
-  //     && AESEncryption.DecryptedWithKey(key, plaintextSeg[|plaintextSeg| - 1])
-  // }
+  predicate DecryptedSegmentsWithKey(key: seq<uint8>, plaintextSeg: seq<seq<uint8>>)
+  {
+    if plaintextSeg == [] then true else
+      && DecryptedSegmentsWithKey(key, plaintextSeg[..|plaintextSeg| - 1])
+      && AESEncryption.DecryptedWithKey(key, plaintextSeg[|plaintextSeg| - 1])
+  }
 
   // method DecryptNonFramedMessageBody(
   //   rd: Streams.ByteReader,
